# 2-6

$A \perp B \mid C$ は

$$
\begin{align}
\Pr(A \cap B \mid C) = \Pr(A \mid C)\Pr(B \mid C)
\end{align} \tag{1}
$$

と表せる

$$
\begin{align}
\Pr(B \mid C) = \Pr(A \cap B \mid C) + \Pr(A^c \cap B \mid C)
\end{align} \tag{2}
$$

より

$$
\begin{align}
\Pr(A^c \cap B \mid C) &= \Pr(B \mid C) - \Pr(A \cap B \mid C) \quad \text{(∵ (2))} \\
&= \Pr(B \mid C) - \Pr(A \mid C)\Pr(B \mid C) \quad \text{(∵ (1))} \\
&= \Pr(B \mid C)(1 - \Pr(A \mid C)) \\
&= \Pr(A^c \mid C)\Pr(B \mid C)
\end{align} \tag{3}
$$

以上より $A^c \perp B \mid C$

同様に

$$
\begin{align}
\Pr(A \cap B^c \mid C) &= \Pr(A \mid C) - \Pr(A \cap B \mid C) \\
&= \Pr(A \mid C) - \Pr(A \mid C)\Pr(B \mid C) \quad \text{(∵ (1))} \\
&= \Pr(A \mid C)(1 - \Pr(B \mid C)) \\
&= \Pr(A \mid C)\Pr(B^c \mid C)
\end{align} \tag{4}
$$

以上より $A \perp B^c \mid C$

さらに同様に

$$
\begin{align}
\Pr(A^c \cap B^c \mid C) &= \Pr(A^c \mid C) - \Pr(A^c \cap B \mid C) \\
&= \Pr(A^c \mid C) - \Pr(A^c \mid C)\Pr(B \mid C) \quad \text{(∵ (3))} \\
&= \Pr(A^c \mid C)(1 - \Pr(B \mid C)) \\
&= \Pr(A^c \mid C)\Pr(B^c \mid C)
\end{align} \tag{5}
$$

以上より $A^c \perp B^c \mid C$

# 3-6

# 3-12
